proofs

code/experimental/ed25519/Hacl.Impl.Ed25519.Sign.Steps.fst
@@ -6,7 +6,6 @@ open FStar.Buffer
 open FStar.UInt32
 
 open Hacl.Impl.Ed25519.ExtPoint
-open Hacl.Impl.Ed25519.Ladder.Step
 
 
 let hint8_p = buffer Hacl.UInt8.t
@@ -182,7 +181,7 @@ val sign_step_2:
       as_seq h (Buffer.sub tmp_bytes 64ul len) == as_seq h msg))
     (ensures (fun h0 _ h1 -> live h0 signature /\ live h0 msg /\ live h0 secret /\
       live h0 tmp_bytes /\ live h1 tmp_bytes /\ live h0 tmp_ints /\ live h1 tmp_ints /\
-      live h1 signature /\ modifies_2 tmp_bytes tmp_ints h0 h1 /\ (
+      live h1 signature /\ modifies_1 tmp_ints h0 h1 /\ (
         let r    = Buffer.sub tmp_ints 20ul 5ul  in
         let prefix_at_message = Buffer.sub tmp_bytes 0ul FStar.UInt32.(64ul +^ len) in
         let tmp_bytes         = Buffer.offset tmp_bytes FStar.UInt32.(64ul +^ len) in
@@ -199,16 +198,7 @@ val sign_step_2:
     ))
 
 
-#reset-options "--max_fuel 0 --z3rlimit 500"
-
-
-let lemma_sub (len:UInt32.t) (tmp:buffer Hacl.UInt8.t{length tmp = 352 + v len}) : Lemma
-  (let prefix_at_message = Buffer.sub tmp 0ul FStar.UInt32.(64ul +^ len) in
-   let prefix_at_msg     = Buffer.sub prefix_at_message 32ul FStar.UInt32.(32ul +^ len) in
-   let message           = Buffer.sub prefix_at_msg 32ul len in
-   message == Buffer.sub tmp 64ul len)
-   = ()
-
+#reset-options "--max_fuel 0 --z3rlimit 20"
 
 let sign_step_2 signature secret msg len g tmp_bytes tmp_ints =
   let tmp_bytes' = tmp_bytes in
@@ -223,27 +213,20 @@ let sign_step_2 signature secret msg len g tmp_bytes tmp_ints =
   let prefix_at_msg = Buffer.sub prefix_at_message 32ul FStar.UInt32.(32ul +^ len) in
   let message       = Buffer.sub prefix_at_msg 32ul len in
   let prefix'       = Buffer.sub prefix_at_msg 0ul 32ul in
-  (* lemma_sub len tmp_bytes'; *)
-  (* let h0 = ST.get() in *)
-  (* copy_bytes prefix' prefix 32ul; *)
-  (* let h1 = ST.get() in *)
-  (* no_upd_lemma_1 h0 h1 prefix' message; *)
-  (* no_upd_lemma_1 h0 h1 prefix' a; *)
-  (* no_upd_lemma_1 h0 h1 prefix' a''; *)
-  (* lemma_append2 h1 prefix_at_msg 32ul len; *)
-  (* assert(as_seq h1 prefix' == as_seq h0 prefix); *)
-  (* assert(as_seq h1 message == as_seq h0 message); *)
-  (* assert(as_seq h1 prefix_at_msg == FStar.Seq.(as_seq h1 prefix' @| as_seq h1 message)); *)
-  (* assert(as_seq h1 prefix_at_msg == FStar.Seq.(as_seq h0 prefix @| as_seq h0 msg)); *)
-  (* assert(live h1 r); *)
-  (* assert(live h1 prefix_at_msg); *)
-  (* Hacl.Impl.SHA512.ModQ.sha512_modq r prefix_at_msg (len+^32ul); *)
-  Hacl.Impl.SHA512.ModQ.sha512_modq_pre r prefix msg len
-  (* let h2 = ST.get() in *)
-  (* no_upd_lemma_1 h1 h2 r message; *)
-  (* no_upd_lemma_1 h1 h2 r a; *)
-  (* no_upd_lemma_1 h1 h2 r a''; *)
-  (* () *)
+  let h0 = ST.get() in
+  Hacl.Impl.SHA512.ModQ.sha512_modq_pre r prefix msg len;
+  let h1 = ST.get() in
+  no_upd_lemma_1 h0 h1 r a;
+  no_upd_lemma_1 h0 h1 r a'';
+  ()
+
+
+(* let lemma_sub (len:UInt32.t) (tmp:buffer Hacl.UInt8.t{length tmp = 352 + v len}) : Lemma *)
+(*   (let prefix_at_message = Buffer.sub tmp 0ul FStar.UInt32.(64ul +^ len) in *)
+(*    let prefix_at_msg     = Buffer.sub prefix_at_message 32ul FStar.UInt32.(32ul +^ len) in *)
+(*    let message           = Buffer.sub prefix_at_msg 32ul len in *)
+(*    message == Buffer.sub tmp 64ul len) *)
+(*    = () *)
 
 
 #reset-options "--max_fuel 0 --z3rlimit 50"
@@ -263,7 +246,7 @@ val sign_step_4:
       as_seq h (Buffer.sub tmp_bytes 64ul len) == as_seq h msg))
     (ensures (fun h0 _ h1 -> live h0 signature /\ live h0 msg /\ live h0 secret /\
       live h0 tmp_bytes /\ live h1 tmp_bytes /\ live h0 tmp_ints /\ live h1 tmp_ints /\
-      live h1 signature /\ modifies_2 tmp_bytes tmp_ints h0 h1 /\ (
+      live h1 signature /\ modifies_1 tmp_ints h0 h1 /\ (
         let tmpa = Buffer.sub tmp_ints 0ul  20ul in
         let r    = Buffer.sub tmp_ints 20ul 5ul  in
         let r'   = Buffer.sub tmp_ints 25ul 20ul in
@@ -292,35 +275,35 @@ val sign_step_4:
 
 #reset-options "--max_fuel 0 --z3rlimit 20"
 
-val append_before_sha:
-  msg:hint8_p ->
-  len:UInt32.t{UInt32.v len = length msg} ->
-  msg':hint8_p{length msg' = 64 + UInt32.v len /\ disjoint msg msg'} ->
-  rs':hint8_p{length rs' = 32 /\ disjoint rs' msg'} ->
-  a'':hint8_p{length a'' = 32 /\ disjoint a'' msg'} ->
-  Stack unit
-    (requires (fun h -> live h msg' /\ live h msg /\ live h rs' /\ live h a'' /\
-      as_seq h (Buffer.sub msg' 64ul len) == as_seq h msg))
-    (ensures (fun h0 _ h1 -> live h1 msg' /\ modifies_1 msg' h0 h1 /\ live h0 msg /\ live h0 rs' /\
-      live h0 a'' /\
-      as_seq h1 msg' == FStar.Seq.(as_seq h0 rs' @| as_seq h0 a'' @| as_seq h0 msg)))
+(* val append_before_sha: *)
+(*   msg:hint8_p -> *)
+(*   len:UInt32.t{UInt32.v len = length msg} -> *)
+(*   msg':hint8_p{length msg' = 64 + UInt32.v len /\ disjoint msg msg'} -> *)
+(*   rs':hint8_p{length rs' = 32 /\ disjoint rs' msg'} -> *)
+(*   a'':hint8_p{length a'' = 32 /\ disjoint a'' msg'} -> *)
+(*   Stack unit *)
+(*     (requires (fun h -> live h msg' /\ live h msg /\ live h rs' /\ live h a'' /\ *)
+(*       as_seq h (Buffer.sub msg' 64ul len) == as_seq h msg)) *)
+(*     (ensures (fun h0 _ h1 -> live h1 msg' /\ modifies_1 msg' h0 h1 /\ live h0 msg /\ live h0 rs' /\ *)
+(*       live h0 a'' /\ *)
+(*       as_seq h1 msg' == FStar.Seq.(as_seq h0 rs' @| as_seq h0 a'' @| as_seq h0 msg))) *)
 
-#reset-options "--max_fuel 0 --z3rlimit 10"
+(* #reset-options "--max_fuel 0 --z3rlimit 10" *)
 
-let append_before_sha msg len msg' rs' a'' =
-  let h0 = ST.get() in
-  copy_bytes (Buffer.sub msg' 0ul 32ul) rs' 32ul;
-  let h1 = ST.get() in
-  no_upd_lemma_1 h0 h1 (Buffer.sub msg' 0ul 32ul) (Buffer.sub msg' 64ul len);
-  no_upd_lemma_1 h0 h1 (Buffer.sub msg' 0ul 32ul) a'';
-  copy_bytes (Buffer.sub msg' 32ul 32ul) a'' 32ul;
-  let h2 = ST.get() in
-  no_upd_lemma_1 h1 h2 (Buffer.sub msg' 32ul 32ul) (Buffer.sub msg' 64ul len);
-  no_upd_lemma_1 h1 h2 (Buffer.sub msg' 32ul 32ul) (Buffer.sub msg' 0ul 32ul);
-  lemma_append h2 msg' 32ul 32ul len
+(* let append_before_sha msg len msg' rs' a'' = *)
+(*   let h0 = ST.get() in *)
+(*   copy_bytes (Buffer.sub msg' 0ul 32ul) rs' 32ul; *)
+(*   let h1 = ST.get() in *)
+(*   no_upd_lemma_1 h0 h1 (Buffer.sub msg' 0ul 32ul) (Buffer.sub msg' 64ul len); *)
+(*   no_upd_lemma_1 h0 h1 (Buffer.sub msg' 0ul 32ul) a''; *)
+(*   copy_bytes (Buffer.sub msg' 32ul 32ul) a'' 32ul; *)
+(*   let h2 = ST.get() in *)
+(*   no_upd_lemma_1 h1 h2 (Buffer.sub msg' 32ul 32ul) (Buffer.sub msg' 64ul len); *)
+(*   no_upd_lemma_1 h1 h2 (Buffer.sub msg' 32ul 32ul) (Buffer.sub msg' 0ul 32ul); *)
+(*   lemma_append h2 msg' 32ul 32ul len *)
 
 
-#reset-options "--max_fuel 0 --z3rlimit 200"
+(* #reset-options "--max_fuel 0 --z3rlimit 200" *)
 
 let sign_step_4 signature secret msg len g tmp_bytes tmp_ints =
   let tmp_bytes' = tmp_bytes in
@@ -337,21 +320,69 @@ let sign_step_4 signature secret msg len g tmp_bytes tmp_ints =
   let rs_bytes = Buffer.sub prefix_at_message 0ul  32ul in
   let a_bytes  = Buffer.sub prefix_at_message 32ul 32ul in
   let message = Buffer.sub prefix_at_message 64ul len in
-  (* lemma_sub len tmp_bytes'; *)
-  (* let h0 = ST.get() in *)
-  (* assume(as_seq h0 (Buffer.sub prefix_at_message 64ul len) == as_seq h0 msg); *)
-  (* append_before_sha msg len prefix_at_message rs' a''; *)
-  (* let h1 = ST.get() in *)
-  (* no_upd_lemma_1 h0 h1 prefix_at_message a; *)
-  (* no_upd_lemma_1 h0 h1 prefix_at_message rs'; *)
-  (* no_upd_lemma_1 h0 h1 prefix_at_message r; *)
-  (* Hacl.Impl.SHA512.ModQ.sha512_modq h prefix_at_message (len+^64ul); *)
-  Hacl.Impl.SHA512.ModQ.sha512_modq_pre_pre2 h rs' a'' msg len
-  (* let h2 = ST.get() in *)
-  (* no_upd_lemma_1 h1 h2 h a; *)
-  (* no_upd_lemma_1 h1 h2 h rs'; *)
-  (* no_upd_lemma_1 h1 h2 h r *)
+  let h0 = ST.get() in
+  Hacl.Impl.SHA512.ModQ.sha512_modq_pre_pre2 h rs' a'' msg len;
+  let h1 = ST.get() in
+  no_upd_lemma_1 h0 h1 h r;
+  no_upd_lemma_1 h0 h1 h rs';
+  no_upd_lemma_1 h0 h1 h a;
+  ()
 
+
+#reset-options "--max_fuel 0 --z3rlimit 20"
+
+val point_mul_g:
+  result:point ->
+  scalar:buffer Hacl.UInt8.t{length scalar = 32 /\ disjoint result scalar} ->
+  Stack unit
+  (requires (fun h -> Buffer.live h scalar /\ live h result))
+  (ensures (fun h0 _ h1 -> Buffer.live h0 scalar /\ live h0 result /\
+    live h1 result /\ modifies_1 result h0 h1 /\ point_inv h1 result /\
+    (let r = as_point h1 result in
+     let n  = as_seq h0 scalar in
+     r == Spec.Ed25519.point_mul n Spec.Ed25519.g) ))
+
+#reset-options "--max_fuel 0 --z3rlimit 20"
+
+let point_mul_g result scalar =
+  push_frame();
+  let h0 = ST.get() in
+  let g = create 0uL 20ul in
+  Hacl.Impl.Ed25519.G.make_g g;
+  let h1 = ST.get() in
+  no_upd_lemma_0 h0 h1 scalar;
+  Hacl.Impl.Ed25519.Ladder.point_mul result scalar g;
+  let h2 = ST.get() in
+  no_upd_lemma_1 h1 h2 result scalar;
+  pop_frame()
+
+
+#reset-options "--max_fuel 0 --z3rlimit 20"
+
+[@ "substitute"]
+val point_mul_g_compress:
+  out:hint8_p{length out = 32} ->
+  s:hint8_p{length s = 32 /\ disjoint s out} ->
+  Stack unit
+    (requires (fun h -> live h out /\ live h s))
+    (ensures (fun h0 _ h1 -> live h1 out /\ live h0 s /\ modifies_1 out h0 h1 /\ live h1 s /\
+      h1.[out] == Spec.Ed25519.(point_compress (point_mul h0.[s] g))))
+
+#reset-options "--max_fuel 0 --z3rlimit 200"
+
+let point_mul_g_compress out s =
+  let h = ST.get() in
+  push_frame();
+  let h0 = ST.get() in
+  let tmp:point = Buffer.create 0uL 20ul in
+  let h' = ST.get() in
+  point_mul_g tmp s;
+  let h1 = ST.get() in
+  no_upd_lemma_0 h0 h1 s;
+  Hacl.Impl.Ed25519.PointCompress.point_compress out tmp;
+  let h2 = ST.get() in
+  no_upd_lemma_1 h1 h2 out s;
+  pop_frame()
 
 #reset-options "--max_fuel 0 --z3rlimit 20"
 
@@ -360,20 +391,20 @@ val sign_step_3:
   secret:hint8_p{length secret = 32} ->
   msg:hint8_p{length msg < pow2 32 - 64} ->
   len:UInt32.t{UInt32.v len = length msg} ->
-  g:point ->
-  tmp_bytes:hint8_p{length tmp_bytes = 352 + UInt32.v len /\ disjoint tmp_bytes signature /\ disjoint tmp_bytes secret /\ disjoint tmp_bytes msg /\ disjoint tmp_bytes g} ->
-  tmp_ints:buffer Hacl.UInt64.t{length tmp_ints = 65 /\ disjoint tmp_bytes tmp_ints /\ disjoint tmp_ints signature /\ disjoint tmp_ints secret /\ disjoint tmp_ints msg /\ disjoint tmp_ints g} ->
+  tmp_bytes:hint8_p{length tmp_bytes = 352 + UInt32.v len /\ disjoint tmp_bytes signature /\ disjoint tmp_bytes secret /\ disjoint tmp_bytes msg} ->
+  tmp_ints:buffer Hacl.UInt64.t{length tmp_ints = 65 /\ disjoint tmp_bytes tmp_ints /\ disjoint tmp_ints signature /\ disjoint tmp_ints secret /\ disjoint tmp_ints msg} ->
   Stack unit
-    (requires (fun h -> live h signature /\ live h msg /\ live h secret /\ live h g /\
-      live h tmp_bytes /\ live h tmp_ints /\ as_point h g == Spec.Ed25519.g /\
+    (requires (fun h -> live h signature /\ live h msg /\ live h secret /\
+      live h tmp_bytes /\ live h tmp_ints /\
       as_seq h (Buffer.sub tmp_bytes 64ul len) == as_seq h msg /\ (
-        let r    = Buffer.sub tmp_ints 20ul 5ul  in
-        Hacl.Spec.BignumQ.Eval.eval_q (as_seq h r) < pow2 256)
+        let s = as_seq h (Buffer.sub tmp_ints 20ul 5ul) in
+        Hacl.Spec.BignumQ.Eval.eval_q s < pow2 256 /\ Hacl.UInt64.v (Seq.index s 0) < pow2 56 /\
+        Hacl.UInt64.v (Seq.index s 1) < pow2 56 /\ Hacl.UInt64.v (Seq.index s 2) < pow2 56 /\
+        Hacl.UInt64.v (Seq.index s 3) < pow2 56 /\ Hacl.UInt64.v (Seq.index s 4) < pow2 32)
       ))
-    (ensures (fun h0 _ h1 -> live h0 signature /\ live h0 msg /\ live h0 secret /\ live h0 g /\
+    (ensures (fun h0 _ h1 -> live h0 signature /\ live h0 msg /\ live h0 secret /\
       live h0 tmp_bytes /\ live h1 tmp_bytes /\ live h0 tmp_ints /\ live h1 tmp_ints /\
       live h1 signature /\ modifies_1 tmp_bytes h0 h1 /\ (
-        let g' = g in
         let tmpa = Buffer.sub tmp_ints 0ul  20ul in
         let r    = Buffer.sub tmp_ints 20ul 5ul  in
         let r'   = Buffer.sub tmp_ints 25ul 20ul in
@@ -394,46 +425,51 @@ val sign_step_3:
         Hacl.Spec.BignumQ.Eval.eval_q (as_seq h0 r) < pow2 256 /\
         as_seq h1 rs' == Spec.Ed25519.(
             let r = Hacl.Spec.BignumQ.Eval.eval_q (as_seq h0 r) in
-            let x = point_mul (Endianness.little_bytes 32ul r) (as_point h0 g') in
+            let x = point_mul (Endianness.little_bytes 32ul r) g in
             point_compress x) /\
         as_seq h1 r == as_seq h0 r
         )
     ))
 
-let sign_step_3 signature secret msg len g tmp_bytes tmp_ints =
+#reset-options "--max_fuel 0 --z3rlimit 100"
+
+let sign_step_3 signature secret msg len tmp_bytes tmp_ints =
   push_frame();
   let h0 = ST.get() in
   let rb = create 0uy 32ul in
   let h1 = ST.get() in
   let r    = Buffer.sub tmp_ints 20ul 5ul  in
+  no_upd_lemma_0 h0 h1 r;
   let tmp_bytes         = Buffer.offset tmp_bytes FStar.UInt32.(64ul +^ len) in
   let rs'  = Buffer.sub tmp_bytes 160ul 32ul in  
   Hacl.Impl.Store56.store_56 rb r;
   let h2 = ST.get() in
+  Endianness.lemma_little_endian_inj (as_seq h2 rb)
+                                     (Endianness.little_bytes 32ul (Hacl.Spec.BignumQ.Eval.eval_q (as_seq h0 r)));
   no_upd_lemma_0 h0 h2 r;
   no_upd_lemma_0 h0 h2 signature;
-  no_upd_lemma_0 h0 h2 g;
   no_upd_lemma_0 h0 h2 tmp_ints;
-  point_mul_compress rs' rb g;
+  point_mul_g_compress rs' rb;
   let h3 = ST.get() in
+  no_upd_lemma_1 h2 h3 rs' r;
   pop_frame()
 
 
+#reset-options "--max_fuel 0 --z3rlimit 20"
+
 val sign_step_5:
-  signature:hint8_p{length signature = 64} ->
-  secret:hint8_p{length secret = 32} ->
-  msg:hint8_p{length msg < pow2 32 - 64} ->
-  len:UInt32.t{UInt32.v len = length msg} ->
-  g:point ->
-  tmp_bytes:hint8_p{length tmp_bytes = 352 + UInt32.v len /\ disjoint tmp_bytes signature /\ disjoint tmp_bytes secret /\ disjoint tmp_bytes msg /\ disjoint tmp_bytes g} ->
-  tmp_ints:buffer Hacl.UInt64.t{length tmp_ints = 65 /\ disjoint tmp_bytes tmp_ints /\ disjoint tmp_ints signature /\ disjoint tmp_ints secret /\ disjoint tmp_ints msg /\ disjoint tmp_ints g} ->
+  len:UInt32.t ->
+  tmp_bytes:hint8_p{length tmp_bytes = 352 + UInt32.v len} ->
+  tmp_ints:buffer Hacl.UInt64.t{length tmp_ints = 65 /\ disjoint tmp_bytes tmp_ints} ->
   Stack unit
-    (requires (fun h -> live h signature /\ live h msg /\ live h secret /\ live h g /\
-      live h tmp_bytes /\ live h tmp_ints /\ as_point h g == Spec.Ed25519.g /\
-      as_seq h (Buffer.sub tmp_bytes 64ul len) == as_seq h msg))
-    (ensures (fun h0 _ h1 -> live h0 signature /\ live h0 msg /\ live h0 secret /\
-      live h0 tmp_bytes /\ live h1 tmp_bytes /\ live h0 tmp_ints /\ live h1 tmp_ints /\
-      live h1 signature /\ modifies_2 tmp_bytes tmp_ints h0 h1 /\ (
+    (requires (fun h -> live h tmp_bytes /\ live h tmp_ints /\ (
+      let h'    = Buffer.sub tmp_ints 60ul 5ul in
+      let r    = Buffer.sub tmp_ints 20ul 5ul  in
+      Hacl.Impl.BignumQ.Mul.within_56 h r /\ Hacl.Spec.BignumQ.Eval.eval_q (as_seq h r) < 0x1000000000000000000000000000000014def9dea2f79cd65812631a5cf5d3ed /\
+      Hacl.Impl.BignumQ.Mul.within_56 h h' /\ Hacl.Spec.BignumQ.Eval.eval_q (as_seq h h') < pow2 256)
+    ))
+    (ensures (fun h0 _ h1 -> live h0 tmp_bytes /\ live h1 tmp_bytes /\
+      live h0 tmp_ints /\ live h1 tmp_ints /\ modifies_2 tmp_bytes tmp_ints h0 h1 /\ (
         let tmpa = Buffer.sub tmp_ints 0ul  20ul in
         let r    = Buffer.sub tmp_ints 20ul 5ul  in
         let r'   = Buffer.sub tmp_ints 25ul 20ul in
@@ -453,12 +489,17 @@ val sign_step_5:
         let prefix = Buffer.sub apre 32ul 32ul in
         Endianness.little_endian (as_seq h1 s') ==
           Spec.Ed25519.((Hacl.Spec.BignumQ.Eval.eval_q (as_seq h0 r) +
-                          (Hacl.Spec.BignumQ.Eval.eval_q (as_seq h0 h) * (Endianness.little_endian (as_seq h0 a)))) % q) /\
+                          ((Hacl.Spec.BignumQ.Eval.eval_q (as_seq h0 h) * (Endianness.little_endian (as_seq h0 a))) % q)) % q) /\
         as_seq h1 rs' == as_seq h0 rs'
         )
     ))
 
-let sign_step_5 signature secret msg len g tmp_bytes tmp_ints =
+#reset-options "--max_fuel 0 --z3rlimit 200"
+
+let sign_step_5 len tmp_bytes tmp_ints =
+  assert_norm(pow2 56 = 0x100000000000000);
+  assert_norm(Spec.Ed25519.q = 0x1000000000000000000000000000000014def9dea2f79cd65812631a5cf5d3ed);
+  assert_norm(pow2 256 = 0x10000000000000000000000000000000000000000000000000000000000000000);
   let r    = Buffer.sub tmp_ints 20ul 5ul  in
   let aq   = Buffer.sub tmp_ints 45ul 5ul  in
   let ha   = Buffer.sub tmp_ints 50ul 5ul  in
@@ -467,9 +508,25 @@ let sign_step_5 signature secret msg len g tmp_bytes tmp_ints =
   let tmp_bytes         = Buffer.offset tmp_bytes FStar.UInt32.(64ul +^ len) in
   let s'   = Buffer.sub tmp_bytes 192ul 32ul in
   let apre = Buffer.sub tmp_bytes 224ul 64ul in
+  let rs'  = Buffer.sub tmp_bytes 160ul 32ul in
   let a      = Buffer.sub apre 0ul 32ul in
+  let h0 = ST.get() in
+  Endianness.lemma_little_endian_is_bounded (as_seq h0 a);
   Hacl.Impl.Load56.load_32_bytes aq a;
+  let h1 = ST.get() in
+  assert(Hacl.Spec.BignumQ.Eval.eval_q (as_seq h1 aq) < pow2 256);
+  no_upd_lemma_1 h0 h1 aq h;
+  no_upd_lemma_1 h0 h1 aq ha;
+  no_upd_lemma_1 h0 h1 aq r;
+  no_upd_lemma_1 h0 h1 aq rs';
   Hacl.Impl.BignumQ.Mul.mul_modq ha h aq;
+  let h2 = ST.get() in
+  no_upd_lemma_1 h1 h2 ha r;
+  no_upd_lemma_1 h1 h2 ha rs';
   Hacl.Impl.BignumQ.Mul.add_modq s r ha;
-  Hacl.Impl.Store56.store_56 s' s
-
+  let h3 = ST.get() in
+  no_upd_lemma_1 h2 h3 s rs';
+  Hacl.Impl.Store56.store_56 s' s;
+  let h4 = ST.get() in
+  no_upd_lemma_1 h3 h4 s' rs';
+  ()
