code/experimental/ed25519/Hacl.Impl.BignumQ.Mul.fsti
@@ -42,7 +42,7 @@ val barrett_reduction:
     (requires (fun h -> live h z /\ live h t /\ (let t = as_seq h t in
       all_10_bellow_56 t /\
       eval_q_10 t.[0] t.[1] t.[2] t.[3] t.[4] t.[5] t.[6] t.[7] t.[8] t.[9] < pow2 512)))
-    (ensures (fun h0 _ h1 -> live h1 z /\ live h0 t /\ (
+    (ensures (fun h0 _ h1 -> live h1 z /\ live h0 t /\ within_56 h1 z /\ (
       let z = as_seq h1 z in
       let t = as_seq h0 t in let op_String_Access = Seq.index in
       all_10_bellow_56 t /\
@@ -61,9 +61,10 @@ val mul_modq:
     (requires (fun h -> live h z /\ live h x /\ live h y /\ within_56 h x /\ within_56 h y /\
       (let x = as_seq h x in let y = as_seq h y in
       eval_q x < pow2 256 /\ eval_q y < pow2 256)))
-    (ensures (fun h0 _ h1 -> live h1 z /\ live h0 x /\ live h0 y /\ 
+    (ensures (fun h0 _ h1 -> live h1 z /\ live h0 x /\ live h0 y /\ modifies_1 z h0 h1 /\
       (let x = as_seq h0 x in let y = as_seq h0 y in
        eval_q x < pow2 256 /\ eval_q y < pow2 256) /\
+       within_56 h1 z /\
        eval_q (as_seq h1 z) == (eval_q (as_seq h0 x) * eval_q (as_seq h0 y)) % 0x1000000000000000000000000000000014def9dea2f79cd65812631a5cf5d3ed))
 
 
@@ -76,8 +77,9 @@ val add_modq:
       (let x = as_seq h x in let y = as_seq h y in
       eval_q x < 0x1000000000000000000000000000000014def9dea2f79cd65812631a5cf5d3ed /\
       eval_q y < 0x1000000000000000000000000000000014def9dea2f79cd65812631a5cf5d3ed)))
-    (ensures (fun h0 _ h1 -> live h1 z /\ live h0 x /\ live h0 y /\ 
+    (ensures (fun h0 _ h1 -> live h1 z /\ live h0 x /\ live h0 y /\ modifies_1 z h0 h1 /\
       (let x = as_seq h0 x in let y = as_seq h0 y in
        eval_q x < 0x1000000000000000000000000000000014def9dea2f79cd65812631a5cf5d3ed /\
        eval_q y < 0x1000000000000000000000000000000014def9dea2f79cd65812631a5cf5d3ed) /\
+       within_56 h1 z /\
        eval_q (as_seq h1 z) == (eval_q (as_seq h0 x) + eval_q (as_seq h0 y)) % 0x1000000000000000000000000000000014def9dea2f79cd65812631a5cf5d3ed))
